started theorem

trans.v
@@ -4,13 +4,19 @@ From istari Require Import Sigma Tactics
      Syntax Subst SimpSub Promote Hygiene
      ContextHygiene Equivalence Rules Defined.
 
+(*movegamma almost definitely wrong because it assumes Gamma starts from beginning of
+ context (var 0) where as there's probably more stuff at the end
+ probably need to pass in a starting index to move Gamma
+ best to work this out when you can test in real time whether its working when you're
+ at there in a proof*)
+
 (*functions which take in the world and give you the type*)
 (*make_ref: tau in source -> (translation of ref tau into target)*)
 Fixpoint  trans_type (W: Syntax.term False) (tau : source.term) {struct tau}: (Syntax.term False)
   :=  match tau with
         nattp_m => nattp
       | unittp_m => unittp
-      | arrow_m A B => all preworld nzero (pi nattp (*u = 1, l = 0*)
+      | arrow_m A B => all preworld nzero (pi nattp (*u := 1, l := 0*)
                                         (let u := var 1 in
                                         let l := var 0 in
                                         let U := ppair u l in
@@ -40,7 +46,7 @@ Fixpoint  trans_type (W: Syntax.term False) (tau : source.term) {struct tau}: (S
                                                        let U := (ppair u l) in
     arrow (subseq W U) (arrow (store U)
                          (laters (exist world nzero ((*u:= 2, l:= 1, v:= 0*)
-                                          sigma nattp (*u = 3, l = 2, v= 1, lv = 0*)
+                                          sigma nattp (*u := 3, l := 2, v= 1, lv := 0*)
                                           (let u := Syntax.var 3 in
                                               let l := Syntax.var 2 in
                                               let v := Syntax.var 1 in
@@ -54,6 +60,11 @@ Fixpoint  trans_type (W: Syntax.term False) (tau : source.term) {struct tau}: (S
                       ))
       | _ => nattp end.
 
+Definition picomp1 (M: term False) := ppi1 M. 
+Definition picomp2 (M: term False) := ppi1 (ppi1 (ppi2 M) ). 
+Definition picomp3 (M: term False) := ppi2 (ppi1 (ppi2 M)). 
+Definition picomp4 (M: term False) := ppi2 (ppi2 M). 
+
 Fixpoint gamma_at (gamma: source.context) (W: Syntax.term False) :=
   map (trans_type W) gamma.
 
@@ -66,48 +77,89 @@ Fixpoint gamma_at (gamma: source.context) (W: Syntax.term False) :=
 (*probably want to make the above a function also so that
  Gamma @ w can be calculated*)
 
-Inductive trans: source.context -> source.term -> (Syntax.term False) -> Type :=
-  t_ref: forall G E Es T, trans G E Es ->
-         of_m G E T ->
-         trans G (ref_m E)
-               (lam ( (*l1  = 0*) lam (*l1 = 1, l = 0*)
-                    ( lam (*l1 = 2, l = 1, m = 0*)
-                       (  lam (*l1 = 3, l = 2, m = 1, s = 0*)
+Definition make_bind E1 E2 := app (app bind E1) E2.
+
+(*every time you put stuff under a lambda you probably have to shift it*)
+Inductive trans: source.term -> (Syntax.term False) -> Type :=
+  t_bind: forall G E1 Et1 E2 Et2 T1 T2, of_m G E1 (comp_m T1) ->
+                                  of_m (cons T1 G) E2 (comp_m T2) ->
+                                   trans E1 Et1 ->
+                                   trans E2 Et2 ->
+                                   trans (bind_m E1 E2)(
+lam ( (*l1 := 0*) lam ( (*l1 := 1, l :=0 *) lam ( (*l1 := 2, l := 1, m := 0*)
+                           lam ( (*l1 := 3, l := 2, m := 1, s := 0*)
+                               let l1 := (var 3) in
+                               let l := (var 2) in
+                               let m := (var 1) in
+                               let s := (var 0) in
+let btarg := app (app (app (app Et1 l1) l) m) s in
+make_bind btarg ( lam (*l1 := 4, l := 3, m := 2, s := 1, z1 := 0*)
+              (
+                               let z1 := (var 0) in (*basically added 5 vars to my context*)
+                               let lv := (picomp1 z1) in
+                               let mv := (picomp2 z1) in
+                               let sv := (picomp3 z1) in
+                               let x' := (picomp4 z1) in
+                               let btarg := app (lam (
+                                               move_gamma G (make_subseq) (*G is almost definitely
+                                                                           the wrong context to put here*)
+                                                          (app (subst (sh 6) Et2) lv))) x' in
+                               let e2bar' := app (app (app btarg lv) make_subseq) sv in
+                               (*start here*)
+                               make_bind e2bar' (lam (
+                                                    let z2 := (var 0) in
+                                                    app ret (ppair (picomp1 z2)
+                                                                   (ppair make_subseq (*z2 \circ z1*)
+                                                        (ppair (picomp3 z2) (picomp4 z2))                         
+                                                        ))
+                                               ))
+              )
+
+          )
+
+    ))
+                                         )))
+  | t_ref: forall G E Et T, 
+         of_m G E T -> trans E Et ->
+         trans (ref_m E)
+               (lam ( (*l1  := 0*) lam (*l1 := 1, l := 0*)
+                    ( lam (*l1 := 2, l := 1, m := 0*)
+                       (  lam (*l1 := 3, l := 2, m := 1, s := 0*)
                             ( let l1 := var 3 in
                               let l := var 2 in
-                             let x := app Es l1 in (*all of Es is @ u1 including vars in Gamma*)
+                             let x := app Et l1 in (*all of Et is @ u1 including vars in Gamma*)
                              let m1 := make_subseq (*u <= u1*) in
                              let p1 := ppair m1 (*store u1*)
                                                (lam (*l2*) 
  (*
-l1 = 4
-l = 3
-m: w <= u = 2
-s: store u, l = 1
-l2: = 0*)                                                
+l1 := 4
+l := 3
+m: w <= u := 2
+s: store u, l := 1
+l2: := 0*)                                                
                              (lam (*m2*)     
  (*
-l1 = 5
-l = 4
-m: w <= u = 3
-s: store u, l = 2
-l2: = 1
-  m2: u1 <= u2 = 0*)                                                
+l1 := 5
+l := 4
+m: w <= u := 3
+s: store u, l := 2
+l2: := 1
+  m2: u1 <= u2 := 0*)                                                
                ( lam (*i*)
  (*
-l1 = 6
-l = 5
-m: w <= u = 4
-s: store u, l = 3
-l2: = 2
-  m2: u1 <= u2 = 1
-  i = 0*)                                                
+l1 := 6
+l := 5
+m: w <= u := 4
+s: store u, l := 3
+l2: := 2
+  m2: u1 <= u2 := 1
+  i := 0*)                                                
                  (let l1 := var 6 in
                  let l := var 5 in
                  let s := var 3 in
                  let l2 := var 2 in
                  let i := var 0 in
-                 let x := app Es l1 in (*all of Es is @ u1 including vars in Gamma*)
+                 let x := app Et l1 in (*all of Et is @ u1 including vars in Gamma*)
                let m1 := make_subseq (*u <= u1*) in
                let m12 := make_subseq in (*compose_sub m2 m1 *)
                let m02 := make_subseq in (*compose_sub m12 m *)
@@ -125,3 +177,4 @@ l2: = 2
                             )
                     ))))
                       ) ).
+
