proofs.v
@@ -1,0 +1,12 @@
+From Coq.Lists Require Import List.
+From istari Require Import source subst_src rules_src help trans.
+From istari Require Import Sigma Tactics
+     Syntax Subst SimpSub Promote Hygiene
+     ContextHygiene Equivalence Rules Defined.
+Check context.
+
+Theorem one: forall G D e T ebar w1 l1,
+    of_m G e T -> tr D (oof (ppair w1 l1) world) ->
+    trans e ebar -> 
+         tr ((gamma_at G (ppair w1 l1)) ++ D) (app ebar (sh (length G) l1))
+            (trans_type T (ppair w1 l1)).
